move Rationals.v into theory/Utils folder

theory/System/PathORAM.v
@@ -10,77 +10,7 @@ Require Import POram.Utils.Classes.
 Import MonadNotation.
 Require Import POram.Utils.Lists.
 Require Import POram.Utils.Vectors.
-(*** RATIONALS ***)
-#[export] Instance Monoid_rat : Monoid Q:= { null := 0 / 1 ; append := Qplus}.
-
-(* DICTIONARIES *)
-
-(* Probably switch to `Coq.FSets.FMaps` or `ExtLib.Map.FMapAList` in a real
- * development. Rolling your own is easy enough to do, and if you go this route
- * you may want to enforce well-formedness and/or decideable equality of the key
- * space via type classes.
- *)
-
-Record dict (K V : Type) := Dict { dict_elems : list (K * V) }.
-Arguments Dict {K V} _.
-Arguments dict_elems {K V} _.
-
-Fixpoint map_alist {K V V' : Type} (f : V -> V') (kvs : list (K * V)) : list (K * V') :=
-  match kvs with
-  | nil => nil
-  | cons (k , v) kvs' => cons (k , f v) (map_alist f kvs')
-  end.
-
-Fixpoint lookup_alist {K V : Type} `{Ord K} (v : V) (k : K) (kvs : list (K * V)) :=
-  match kvs with
-  | nil => v
-  | cons (k' , v') kvs' => match ord_dec k k' with
-    | Lt => lookup_alist v k kvs'
-    | Eq => v'
-    | Gt => lookup_alist v k kvs'
-    end
-  end.
-
-Inductive wf_dict_falist {K V : Type} `{Ord K} : forall (kO : option K) (kvs : list (K * V)), Prop :=
-  | nil_WFDict : forall {kO : option K}, wf_dict_falist kO []
-  | cons_WFDict : forall {kO : option K} {k : K} {v : V} {kvs : list (K * V)},
-      match kO return Set with
-      | None => unit
-      | Some k' => ord_dec k' k = Lt
-      end
-      -> wf_dict_falist (Some k) kvs
-      -> wf_dict_falist kO ((k , v) :: kvs).
-
-Fixpoint lookup_falist {K V : Type} `{Ord K} (v : V) (k : K) (kvs : list (K * V)) :=
-  match kvs with
-  | nil => v
-  | cons (k' , v') kvs' => match ord_dec k k' with
-    | Lt => v
-    | Eq => v'
-    | Gt => lookup_falist v k kvs'
-    end
-  end.
-
-Fixpoint update_falist {K V : Type} `{Ord K} (k : K) (v : V) (kvs : list (K * V)) : list (K * V) :=
-  match kvs with
-  | nil => [ (k , v) ]
-  | cons (k' , v') kvs' => match ord_dec k k' with
-      | Lt => (k , v) :: (k' , v') :: kvs'
-      | Eq => (k , v) :: kvs'
-      | Gt => (k' , v') :: update_falist k v kvs'
-      end
-  end.
-
-#[export] Instance WF_dict {K V : Type} `{Ord K} : WF (dict K V) := { wf kvs := wf_dict_falist None (dict_elems kvs) }.
-
-#[export] Instance Functor_dict {K : Type} : Functor (dict K) :=
-  { map {_ _} f kvs := Dict (map_alist f (dict_elems kvs)) }.
-
-Definition lookup_dict {K V : Type} `{Ord K} (v : V) (k : K) (kvs : dict K V) := lookup_falist v k (dict_elems kvs).
-
-Definition update_dict {K V : Type} `{Ord K} (k : K) (v : V) (kvs : dict K V) : dict K V :=
-  Dict (update_falist k v (dict_elems kvs)).
-
+Require Import POram.Utils.Rationals.
 (*** DISTRIBUTIONS ***)
 
 (* You may need to just roll your own on this one, and it will be a pain. This
@@ -2547,7 +2477,7 @@ Proof.
   unfold lookup_dict.
   unfold update_dict.
   destruct m; simpl.
-  induction dict_elems0 as [|[k v] tl]; simpl.
+  induction dict_elems as [|[k v] tl]; simpl.
   - rewrite Nat.compare_refl; auto.
   - destruct (id ?= k)%nat eqn:id_cond; simpl.
     + rewrite Nat.compare_refl; auto.
@@ -2567,7 +2497,7 @@ Proof.
   unfold lookup_dict.
   unfold update_dict.
   destruct m; simpl.
-  induction dict_elems0 as [|[k v] tl]; simpl.
+  induction dict_elems as [|[k v] tl]; simpl.
   - destruct (id ?= id')%nat eqn:id_cond; auto.
     rewrite Nat.compare_eq_iff in id_cond; contradiction.
   - destruct (id' ?= k)%nat eqn:id_cond1; simpl.
